coq-SystemRF-1.1/Denotations/BasicPropsDenotes.v
@@ -1,0 +1,35 @@
+Require Import SystemRF.BasicDefinitions.
+Require Import SystemRF.Names.
+Require Import SystemRF.Strengthenings.
+Require Import SystemRF.Semantics.
+Require Import SystemRF.SystemFTyping.
+Require Import SystemRF.WellFormedness.
+Require Import SystemRF.BasicPropsSubstitution.
+Require Import SystemRF.BasicPropsEnvironments.
+Require Import SystemRF.BasicPropsWellFormedness.
+Require Import Denotations.ClosingSubstitutions.
+Require Import Denotations.Denotations.
+Require Import Denotations.BasicPropsCSubst.
+
+Lemma lem_denotesenv_loc_closed : forall (g:env) (th:csub), 
+    DenotesEnv g th -> loc_closed th.
+Proof. intros; induction H; simpl; try split; trivial.
+  - (* CCons *) apply lem_den_hasftype in H1; 
+    apply lem_ftyp_islc in H1; assumption.
+  - (* CConsT *) apply lem_wftype_islct in H2; assumption. 
+  Qed.
+
+Lemma lem_denotesenv_closed : forall (g:env) (th:csub), 
+    DenotesEnv g th -> closed th.
+Proof. intros; induction H; simpl; trivial.
+  - (* CCons *) apply lem_den_hasftype in H1;
+    apply lem_fv_subset_bindsF in H1; repeat split;
+    try apply IHDenotesEnv; apply no_elem_empty; intuition.
+  - (* CConsT *) apply lem_free_subset_binds in H2;repeat split;
+    try apply IHDenotesEnv; apply no_elem_empty; intuition.
+  Qed.
+
+Lemma lem_denotesenv_substitutable : forall (g:env) (th:csub), 
+    DenotesEnv g th -> substitutable th.
+Proof. intros; induction H; simpl; try split; trivial.
+  apply lem_den_isvalue with (ctsubst th t); apply H1. Qed.
