coq-SystemRF-1.1/Denotations/PrimitivesDenotations.v
@@ -9,6 +9,7 @@ Require Import SystemRF.BasicPropsWellFormedness.
 Require Import SystemRF.Typing.
 Require Import Denotations.ClosingSubstitutions.
 Require Import Denotations.Denotations.
+Require Import Denotations.BasicPropsCSubst.
 Require Import Denotations.PrimitivesSemantics.
 
 Require Import Arith.
@@ -171,7 +172,7 @@ Proof. unfold ty; rewrite Denotes_equation_2;
   Qed.  
 
 Lemma lem_den_imp : Denotes (ty Imp) (Prim Imp).
-Proof. unfold ty; rewrite Denotes_equation_2;
+Proof. unfold ty; simpl; rewrite Denotes_equation_2;
   repeat split; unfold tsubBV; simpl; try apply FTPrm; intros.
   assert (isBool v_x)
     by (apply lem_den_bools with (TRefn TBool PEmpty); simpl; trivial).
@@ -272,39 +273,179 @@ Proof. unfold ty; rewrite Denotes_equation_4;
   destruct t_a eqn:Hta; simpl in Heta; try discriminate;
   simpl in H; try contradiction; injection Heta as Heta;
   subst b1; subst t_a.
-  - (* TBool *) exists (Prim Imp); split; simpl;
-    try apply lem_step_evals; try apply lem_step_leql_tbool.
-    
-    pose proof lem_den_imp; simpl in H5; apply H5.
+  - (* TBool *) exists (Prim Imp); split; try split; simpl;
+    try apply lem_step_evals; try apply lem_step_leql_tbool;
+    rewrite Denotes_equation_2; 
+    repeat split; unfold tsubBV; simpl; try apply FTPrm; intros.
+    assert (isBool v_x)
+        by (apply lem_den_bools with (TRefn TBool ps); simpl; trivial).
+    destruct v_x eqn:E; simpl in H1; try contradiction.
+    destruct b1 eqn:B1.
+    * (* Bc true *) exists (Lambda (BV 0)); split; try split;
+      try apply lem_step_evals; try apply lem_step_imp_tt.
+      rewrite Denotes_equation_2; simpl; repeat split;
+      try apply FTAbs with Base empty; try apply WFFTBasic;
+      unfold unbind; unfold tsubBV; simpl; intros;
+      try apply FTVar; unfold bound_inF; auto;
+      assert (isBool v_x0)
+        by (apply lem_den_bools with (TRefn TBool (psubBV_at 1 (Bc true) ps)); 
+            simpl; trivial);
+      destruct v_x0 eqn:E0; try contradiction.
+      exists (Bc b2); repeat split; unfold psubBV; simpl;
+      try apply lem_step_evals; try apply EAppAbs;
+      try apply FTBC; try apply PECons; try apply PEEmp;
+      try apply AddStep with  
+        (App (App (Prim Eqv) (App (App (Prim Imp) (Bc true)) (Bc b2))) (Bc b2));
+      try apply EApp1; try apply EApp2; try apply EApp1; try apply EApp1;
+      try apply lem_step_leql_tbool;
+      try apply lemma_evals_trans with (Bc (Bool.eqb (implb true b2) b2)); 
+      try apply lemma_semantics_refn_imp; destruct b2; simpl; 
+      try apply Refl; auto.
+    * (* Bc false *) exists (Lambda (Bc true)); split; try split;
+      try apply lem_step_evals; try apply lem_step_imp_ff.
+      rewrite Denotes_equation_2; simpl; repeat split;
+      try apply FTAbs with Base empty; try apply WFFTBasic;
+      unfold unbind; unfold tsubBV; simpl; intros;
+      try apply FTBC; trivial. 
+      assert (isBool v_x0)
+        by (apply lem_den_bools with (TRefn TBool (psubBV_at 1 (Bc false) ps)); 
+            simpl; trivial);
+      destruct v_x0 eqn:E0; try contradiction.
+      exists (Bc true); repeat split; unfold psubBV; simpl;
+      try apply lem_step_evals; try apply EAppAbs; try apply H8;
+      try apply FTBC; apply PECons; try apply PEEmp.
+      apply AddStep with  
+        (App (App (Prim Eqv) (App (App (Prim Imp) (Bc false)) (Bc b2))) (Bc true));
+      try apply EApp1; try apply EApp2; try apply EApp1; try apply EApp1;
+      try apply lem_step_leql_tbool;
+      try apply lemma_evals_trans with (Bc (Bool.eqb (implb false b2) true)); 
+      try apply lemma_semantics_refn_imp; destruct b2; try apply Refl; simpl; exact I.  
+  - (* TInt *) exists (Prim Leq); split; try split; simpl;
+    try apply lem_step_evals; try apply lem_step_leql_tint;
+    rewrite Denotes_equation_2; 
+    repeat split; unfold tsubBV; simpl; try apply FTPrm; intros.
+    assert (isInt v_x)
+        by (apply lem_den_ints with (TRefn TInt ps); simpl; trivial).
+    destruct v_x eqn:E; simpl in H1; try contradiction.
+    exists (Prim (Leqn n)); split; try split;
+    try apply lem_step_evals; try apply lem_step_leq.
+    rewrite Denotes_equation_2; simpl; repeat split; 
+    try apply FTPrm; unfold tsubBV; simpl; intros.
+    assert (isInt v_x0)
+      by (apply lem_den_ints with (TRefn TInt (psubBV_at 1 (Ic n) ps)); simpl; trivial);
+    destruct v_x0 eqn:E0; try contradiction.
+    exists (Bc (n <=? n0)); repeat split; unfold psubBV; simpl;
+    try apply lem_step_evals; try apply lem_step_leqn;
+    try apply FTBC; try apply PECons; try apply PEEmp.
+    apply AddStep with  
+        (App (App (Prim Eqv) (App (App (Prim Leq) (Ic n)) (Ic n0))) (Bc (n <=? n0)));
+    try apply EApp1; try apply EApp2; try apply EApp1; try apply EApp1;
+    try apply lem_step_leql_tint;    
+    try apply lemma_evals_trans with (Bc (Bool.eqb (n <=? n0) (n <=? n0)));
+    try apply lemma_semantics_refn_leq;  
+    set (b' := n <=? n0); assert (Bool.eqb b' b' = true)
+      by (pose proof (Bool.eqb_refl b'); destruct (Bool.eqb b' b'); 
+          try contradiction; reflexivity);
+    try rewrite H10; try apply Refl; auto. 
+  Qed.
 
-  - (* TInt *)
+Lemma lem_den_eql : Denotes (ty Eql) (Prim Eql).
+Proof. unfold ty; rewrite Denotes_equation_4;
+  repeat split; unfold tsubBTV; simpl; try apply FTPrm; intros.
+  destruct (erase t_a) eqn:Heta; apply lem_erase_wftype in H0;
+  rewrite Heta in H0; simpl in H0; inversion H0;
+  try (simpl in H3; contradiction);
+  destruct b eqn:B; simpl in H3; try contradiction;
+  destruct t_a eqn:Hta; simpl in Heta; try discriminate;
+  simpl in H; try contradiction; injection Heta as Heta;
+  subst b1; subst t_a.
+  - (* TBool *) exists (Prim Eqv); split; try split; simpl;
+    try apply lem_step_evals; try apply lem_step_eql_tbool;
+    rewrite Denotes_equation_2; 
+    repeat split; unfold tsubBV; simpl; try apply FTPrm; intros.
+    assert (isBool v_x)
+        by (apply lem_den_bools with (TRefn TBool ps); simpl; trivial).
+    destruct v_x eqn:E; simpl in H1; try contradiction.
+    destruct b1 eqn:B1.
+    * (* Bc true *) exists (Lambda (BV 0)); split; try split;
+      try apply lem_step_evals; try apply lem_step_eqv_tt.
+      rewrite Denotes_equation_2; simpl; repeat split;
+      try apply FTAbs with Base empty; try apply WFFTBasic;
+      unfold unbind; unfold tsubBV; simpl; intros;
+      try apply FTVar; unfold bound_inF; auto;
+      assert (isBool v_x0)
+        by (apply lem_den_bools with (TRefn TBool (psubBV_at 1 (Bc true) ps)); 
+            simpl; trivial);
+      destruct v_x0 eqn:E0; try contradiction.
+      exists (Bc b2); repeat split; unfold psubBV; simpl;
+      try apply lem_step_evals; try apply EAppAbs;
+      try apply FTBC; try apply PECons; try apply PEEmp;
+      try apply AddStep with  
+        (App (App (Prim Eqv) (App (App (Prim Eqv) (Bc true)) (Bc b2))) (Bc b2));
+      try apply EApp1; try apply EApp2; try apply EApp1; try apply EApp1;
+      try apply lem_step_eql_tbool;
+      try apply lemma_evals_trans with (Bc (Bool.eqb (Bool.eqb true b2) b2)); 
+      try apply lemma_semantics_refn_eqv; destruct b2; simpl; 
+      try apply Refl; auto.
+    * (* Bc false *) exists (Prim Not); split; try split;
+      try apply lem_step_evals; try apply lem_step_eqv_ff.
+      rewrite Denotes_equation_2; simpl; repeat split;
+      try apply FTPrm; unfold tsubBV; simpl; intros.
+      assert (isBool v_x0)
+        by (apply lem_den_bools with (TRefn TBool (psubBV_at 1 (Bc false) ps)); 
+            simpl; trivial);
+      destruct v_x0 eqn:E0; try contradiction.
+      exists (Bc (negb b2)); repeat split; unfold psubBV; simpl;
+      try apply lem_step_evals; try apply lem_step_not;
+      try apply FTBC; apply PECons; try apply PEEmp.
+      apply AddStep with  
+        (App (App (Prim Eqv) (App (App (Prim Eqv) (Bc false)) (Bc b2))) (Bc (negb b2)));
+      try apply EApp1; try apply EApp2; try apply EApp1; try apply EApp1;
+      try apply lem_step_eql_tbool;
+      try apply lemma_evals_trans with (Bc (Bool.eqb (Bool.eqb false b2) (negb b2)));
+      try apply lemma_semantics_refn_eqv; destruct b2; try apply Refl; simpl; exact I.  
+  - (* TInt *) exists (Prim Eq); split; try split; simpl;
+    try apply lem_step_evals; try apply lem_step_eql_tint;
+    rewrite Denotes_equation_2; 
+    repeat split; unfold tsubBV; simpl; try apply FTPrm; intros.
+    assert (isInt v_x)
+        by (apply lem_den_ints with (TRefn TInt ps); simpl; trivial).
+    destruct v_x eqn:E; simpl in H1; try contradiction.
+    exists (Prim (Eqn n)); split; try split;
+    try apply lem_step_evals; try apply lem_step_eq.
+    rewrite Denotes_equation_2; simpl; repeat split; 
+    try apply FTPrm; unfold tsubBV; simpl; intros.
+    assert (isInt v_x0)
+      by (apply lem_den_ints with (TRefn TInt (psubBV_at 1 (Ic n) ps)); simpl; trivial);
+    destruct v_x0 eqn:E0; try contradiction.
+    exists (Bc (n =? n0)); repeat split; unfold psubBV; simpl;
+    try apply lem_step_evals; try apply lem_step_eqn;
+    try apply FTBC; try apply PECons; try apply PEEmp.
+    apply AddStep with  
+        (App (App (Prim Eqv) (App (App (Prim Eq) (Ic n)) (Ic n0))) (Bc (n =? n0)));
+    try apply EApp1; try apply EApp2; try apply EApp1; try apply EApp1;
+    try apply lem_step_eql_tint;    
+    try apply lemma_evals_trans with (Bc (Bool.eqb (n =? n0) (n =? n0)));
+    try apply lemma_semantics_refn_eq;  
+    set (b' := n =? n0); assert (Bool.eqb b' b' = true)
+      by (pose proof (Bool.eqb_refl b'); destruct (Bool.eqb b' b'); 
+          try contradiction; reflexivity);
+    try rewrite H10; try apply Refl; auto. 
+  Qed.
 
-  destruct t_a eqn:TA; simpl in H; try contradiction;
-  inversion H0; try (simpl in H5; contradiction). Focus 2.
-
-
-{-@ lem_den_ty :: g:Env -> th:CSub -> ProofOf(DenotesEnv g th)
-        -> c:Prim -> ProofOf(Denotes (ctsubst th (ty c)) (Prim c)) @-}
-lem_den_ty :: Env -> CSub -> DenotesEnv -> Prim -> Denotes
-lem_den_ty g th den_g_th And      = lem_den_and    ? lem_ctsubst_nofree th (ty And)
-lem_den_ty g th den_g_th Or       = lem_den_or     ? lem_ctsubst_nofree th (ty Or)
-lem_den_ty g th den_g_th Not      = lem_den_not () ? lem_ctsubst_nofree th (ty Not)
-lem_den_ty g th den_g_th Eqv      = lem_den_eqv    ? lem_ctsubst_nofree th (ty Eqv)
-lem_den_ty g th den_g_th Leq      = lem_den_leq    ? lem_ctsubst_nofree th (ty Leq)
-lem_den_ty g th den_g_th (Leqn n) = lem_den_leqn n ? lem_ctsubst_nofree th (ty (Leqn n))
-lem_den_ty g th den_g_th Eq       = lem_den_eq     ? lem_ctsubst_nofree th (ty Eq)
-lem_den_ty g th den_g_th (Eqn n)  = lem_den_eqn  n ? lem_ctsubst_nofree th (ty (Eqn n))
-lem_den_ty g th den_g_th Eql      = lem_den_eql () ? lem_ctsubst_nofree th (ty Eql)
-
-
-{-@ lem_denote_sound_typ_tprim :: g:Env -> c:Prim 
-        ->  th:CSub  -> ProofOf(DenotesEnv g th)
-        -> ProofOf(ValueDenoted (csubst th (Prim c)) (ctsubst th (ty c))) @-}
-lem_denote_sound_typ_tprim :: Env -> Prim -> CSub -> DenotesEnv -> ValueDenoted
-lem_denote_sound_typ_tprim g c th den_g_th 
-  = ValDen (Prim c ? lem_csubst_prim th c) (ctsubst th (ty c)) (Prim c ? val_pf ? term_pf) 
-           (Refl (Prim c)) den_tyc_c
-      where
-        den_tyc_c = lem_den_ty g th den_g_th c
-        val_pf    = toProof ( isValue (Prim c) === True )
-        term_pf   = toProof ( isTerm (Prim c) === True )
+Lemma lem_den_ty : forall (g:env) (th:csub) (c:prim),
+    DenotesEnv g th -> Denotes (ctsubst th (ty c)) (Prim c).
+Proof. intros; rewrite lem_ctsubst_nofree; destruct c; 
+  simpl; try reflexivity.
+  - apply lem_den_and.
+  - apply lem_den_or.
+  - apply lem_den_not.
+  - apply lem_den_eqv.
+  - apply lem_den_imp.
+  - apply lem_den_leq.
+  - apply lem_den_leqn.
+  - apply lem_den_eq.
+  - apply lem_den_eqn.
+  - apply lem_den_leql.
+  - apply lem_den_eql.
+  Qed.
