coq-SystemRF-1.1/compile.sh
@@ -83,12 +83,16 @@ echo "Checking Denotations.v ..."
 coqc -Q SystemRF SystemRF -R Denotations Denotations Denotations/Denotations.v
 echo "Checking BasicPropsCSubst.v ..."
 coqc -Q SystemRF SystemRF -R Denotations Denotations Denotations/BasicPropsCSubst.v
+echo "Checking BasicPropsDenotes.v ..."
+coqc -Q SystemRF SystemRF -R Denotations Denotations Denotations/BasicPropsDenotes.v
 echo "Checking BasicPropsSemantics.v ..."
 coqc -Q SystemRF SystemRF -R Denotations Denotations Denotations/BasicPropsSemantics.v
 echo "Checking PrimitivesSemantics.v ..."
 coqc -Q SystemRF SystemRF -R Denotations Denotations Denotations/PrimitivesSemantics.v
 echo "Checking PrimitivesDenotations.v ..."
 coqc -Q SystemRF SystemRF -R Denotations Denotations Denotations/PrimitivesDenotations.v
+echo "Checking SelfifyDenotations.v ..."
+coqc -Q SystemRF SystemRF -R Denotations Denotations Denotations/SelfifyDenotations.v
 echo "Checking DenotationalSoundness.v ..."
 coqc -Q SystemRF SystemRF -R Denotations Denotations Denotations/DenotationalSoundness.v
 echo "Checking MainProperties.v ..."
